\paragraph{a) without characteristic function} \ \\ 
\\
Let $p_x$ and $p_y$ be Gaussian distributions with 
parameters $\mu_x$, $\mu_y$ and $\sigma$.
\begin{equation}
    p_x(x)=\frac{1}{\sqrt{2\pi\sigma}}
    \exp\bigg(-\frac{(x-\mu_x)^2}{2\sigma^2}\bigg)
\end{equation}
\begin{equation}
    p_y(y)=\frac{1}{\sqrt{2\pi\sigma}}
    \exp\bigg(-\frac{(y-\mu_y)^2}{2\sigma^2}\bigg)
\end{equation}
\begin{align}
    p_z(z)
    &=\int dx\int dy\cdot\delta(z-(x+y))\cdot p(x,y) \\
    &=\int dx\int dy\cdot\delta(z-(x+y))\cdot p(x)\cdot p(y) \\
    &=\frac{1}{2\pi\sigma^2}\int dx\int dy\cdot
    \delta(z-(x+y))\cdot
    \exp\bigg(-\frac{(y-\mu_y)^2}{2\sigma^2}\bigg)\cdot
    \exp\bigg(-\frac{(x-\mu_x)^2}{2\sigma^2}\bigg) \\
    &=
    &=\frac{1}{\sqrt{4\pi\sigma^2}}\cdot
    \exp\bigg(-\frac{(z-\mu_x-\mu_y)^2}{4\sigma^2}\bigg)
\end{align}
With $\mu_z=\frac{\mu_x+\mu_y}{2}$
and $\sigma_z=\frac{\sigma}{\sqrt{2}}$, this can be 
rewritten as
\begin{equation}
    p_z(z)
    =\frac{1}{\sqrt{2\pi\sigma_z^2}}\cdot
    \exp\bigg(-\frac{(z/2-\mu_z)^2}{2\sigma^2}\bigg)
\end{equation}
    % \mu_=
    % \sigma_z=
    % \footnote{
    % \url{ en.wikipedia.org/wiki/Sum_of_normally_distributed_random_variables } 
    % }

\paragraph{b) with characteristic function} \ \\

